change subterm funtion

coq/CHLR.v
@@ -2,6 +2,8 @@ Require Import List.
 Import ListNotations.
 Require Import Omega.
 Require Import Bool.
+Require Import Coq.Program.Equality.
+Set Asymmetric Patterns.
 
 (* Role of a subtree w.r.t. its parent node: whether
    it its unique descendant (U), right (R) or left (L)
@@ -55,213 +57,222 @@ Definition AppT' : Term.
                       (BVar [U;U;R] 2 0 _)
                 )
           )
-    ).
-  omega. omega.
-Defined.
-
-Eval compute in AppT'.
-Eval compute in AppT.
-
-Definition exampleC : Term.
-  refine (
-      Lam ([]) 0
-          (App ([U]) 1
-               (App ([U;L]) 1
-                    (Lam ([U;L;L]) 1
-                         (BVar ([U;L;L;U]) 2 1 _))
-                    (Lam ([U;L;R]) 1
-                         (BVar ([U;L;R;U]) 2 1 _))
-               )
-               (Lam ([U;R]) 1 (
-                      App ([U;R;U]) 2 
-                          (BVar ([U;R;U;L]) 2 0 _) 
-                          (BVar ([U;R;U;R]) 2 1 _)))
-               )
     ); omega.
 Defined.
+
+Definition exampleC : Term. 
+  refine (
+      Lam [] 0
+          (App [U] 1
+               (Lam [U;L] 1
+                    (App [U;L;U] 2
+                         (BVar [U;L;U;L] 2 0 _)
+                         (Lam [U;L;U;R] 2 (BVar [U;L;U;R;U] 3 0 _))
+                    )
+               )
+               (Lam [U;R] 1
+                    (App [U;R;U] 2
+                         (BVar [U;R;U;L] 2 1 _)
+                         (BVar [U;R;U;R] 2 0 _)
+                    )
+               )
+          )
+    ); omega.
+Defined.
+
+Eval compute in AppT.
+Eval compute in AppT'.
+Eval compute in exampleC.
 
 (* Auxilliary lemma *)
 Lemma cons_to_app : forall (A : Set) (a : A) (l : list A), a::l = [a] ++ l.
 Proof. auto. Qed.
 
-
 (* Subterm: subterm t p returns a subterm of t, indexed by 
    (relative) path p; if the term does not exists, returns None
 *)
+(* Definition subterm :  *)
+(*   forall {P : Path} {l : nat} (P' : Path), *)
+(*   TermT P l -> option { l' : nat & TermT (P ++ P') l'}. *)
+(*   refine ( *)
+(*       fix subterm' {P : Path} {l : nat} (P' : Path) {struct P'} *)
+(*       : TermT P l -> option { l' : nat & TermT (P ++ P') l'} := *)
+(*         fun T => *)
+(*       match P' return option { l' : nat & TermT (P ++ P') l'} with *)
+(*       | []   => Some _ *)
+(*       | x::p => *)
+(*           match x return option { l' : nat & TermT (P ++ x::p) l'} with *)
+(*           | U => match T return option { l' : nat & TermT (P ++ U::p) l'} with *)
+(*                  | Lam t => _ *)
+(*                  | _     => None *)
+(*                  end *)
+(*           | L => match T return option { l' : nat & TermT (P ++ L::p) l'} with *)
+(*                  | App t _ => _ *)
+(*                  | _       => None *)
+(*                  end *)
+(*           | R => match T return option { l' : nat & TermT (P ++ R::p) l'} with *)
+(*                  | App _ t => _ *)
+(*                  | _       => None *)
+(*                  end *)
+(*         end *)
+(*   end). *)
+(*   exists l; rewrite app_nil_r; apply T. *)
+(*   apply (subterm' (P++[U]) (S l) p) in t. rewrite <- app_assoc in t. assumption. *)
+(*   apply (subterm' (P++[R])  l    p) in t; rewrite <- app_assoc in t; assumption. *)
+(*   apply (subterm' (P++[L])  l    p) in t; rewrite <- app_assoc in t; assumption. *)
+(* Defined. *)
+
 Definition subterm : 
-  forall {P : Path} {l : nat} (P' : Path),
-  TermT P l -> option { l' : nat & TermT (P ++ P') l'}.
+  forall {P P2 : Path} {l : nat} (P' : Path),
+    TermT P l -> P2 = P ++ P' -> option { l' : nat & TermT P2 l'}.
   refine (
-      fix subterm' {P : Path} {l : nat} (P' : Path) {struct P'}
-      : TermT P l -> option { l' : nat & TermT (P ++ P') l'} :=
-        fun T =>
-      match P' return option { l' : nat & TermT (P ++ P') l'} with
-      | []   => Some _
-      | x::p =>
-          match x return option { l' : nat & TermT (P ++ x::p) l'} with
-          | U => match T return option { l' : nat & TermT (P ++ U::p) l'} with
-                 | Lam _ _ t => _
-                 | _     => None
-                 end
-          | L => match T return option { l' : nat & TermT (P ++ L::p) l'} with
-                 | App _ _ t _ => _
-                 | _       => None
-                 end
-          | R => match T return option { l' : nat & TermT (P ++ R::p) l'} with
-                 | App _ _ _ t => _
-                 | _       => None
-                 end
-        end
-  end).
-  exists l. rewrite app_nil_r. apply T.
-  apply (subterm' (P++[U]) (S l) p) in t. rewrite <- app_assoc in t. assumption.
-  apply (subterm' (P++[R])  l    p) in t; rewrite <- app_assoc in t; assumption.
-  apply (subterm' (P++[L])  l    p) in t; rewrite <- app_assoc in t; assumption.
+      fix subterm' {P P2 : Path} {l : nat} (P' : Path) {struct P'}
+      : TermT P l -> P2 = P ++ P'  -> option { l' : nat & TermT P2 l'} :=
+        fun T EQ => _
+    ).
+  induction P'.
+  apply Some; exists l; rewrite app_nil_r in EQ; rewrite EQ; assumption.
+  destruct a.
+  - destruct T.
+    apply (subterm' (P++[U]) P2 (S l) P') in T; [auto | rewrite <- app_assoc];  assumption.
+    apply None.
+    apply None.
+    apply None.
+  - destruct T.
+    apply None.
+    apply (subterm' (P++[R]) P2 l P') in T2; [auto | rewrite <- app_assoc];  assumption.
+    apply None.
+    apply None.
+  - destruct T.
+    apply None.
+    apply (subterm' (P++[L]) P2 l P') in T1; [auto | rewrite <- app_assoc];  assumption.
+    apply None.
+    apply None.
 Defined.
 
-Notation "A [| p |]" := (subterm p A) (at level 0).
+Notation "A [| p |] l1" := (subterm p A l1) (at level 0).
 
-Print subterm.
-Check subterm.
-Eval compute in (AppT) [| [U;U] |].
-Eval compute in (AppT) [|[]|].
-Eval compute in ((AppT) [|[]|] : option {l' : nat & TermT [] l'}).
-Eval cbv in (((AppT) [|[]|] : option {l' : nat & TermT [] l'})).
+Lemma l1 : [U;U] = [U;U] ++ []. auto. Qed.
+Eval compute in AppT [| [U;U] |] l1.
 
-Require Import Coq.Program.Equality.
-
-Theorem AppTEq :
-  ((AppT) [|[]|] : option {l' : nat & TermT ([]) l'}) =
-  Some (existT (fun x => TermT [] x) 0 AppT).
-Proof. simpl_eq; auto. Qed.
-
-Theorem PE :
-  option {l' : nat & TermT ([] ++ []) l'} = option {l' : nat & TermT ([]) l'}.
-Proof. reflexivity. Qed.
-
-Theorem TEq:
-  forall T : Term,
-    (T [|[]|] : option {l' : nat & TermT [] l'}) =
-    Some (existT (fun x => TermT [] x) 0 T).
-Proof. simpl_eq; auto. Qed.
-
-Definition laminPath :
-  Path -> nat.
-  refine(fix laminPath' (p : Path) : nat :=
-           match p with
-             | [] => 0
-             | U :: ps => 1 + laminPath' ps
-             | _ :: ps => laminPath' ps
-           end
-        ).
-Defined.
-
+(* fixpath : by a given P' : Path, l' : nat, and t : TermT P l 
+  returns a TermT P' l' that is a same "term" with a new
+  path and lambda counter.
+  This function will be user futher in linear substitution
+*)
 Definition fixpath :
-  forall {P : Path} {l : nat} (P' : Path) (l' : nat),
+  forall {P : Path} {l : nat} (P' : Path) (l' ll: nat),
     TermT P l -> l' >= l ->TermT P' l'.
   refine(
-      fun P l P' l' t EQ =>
-        let fix fixpath' {P : Path} {l : nat} (t : TermT P l) (l' : nat) (P' : Path) (pr : l' >= l)
+      fun P l P' l' ll t EQ =>
+        let fix fixpath' {P : Path} {l : nat} (t : TermT P l) (l' : nat) (P' : Path) (pr : l' >= l) (ll : nat)
             : TermT P' l' :=
             match t with
-              | Lam _ _ t     => Lam P' l' (fixpath' t (S l') (P' ++ [U]) _)
-              | App _ _ t1 t2 => App P' l' (fixpath' t1 l' (P' ++ [L]) pr) (fixpath' t1 l' (P' ++ [R]) _)
-              | BVar _ _ n eq => BVar P' l' n _
-              | FVar _ _ n    => FVar P' l' n
+              | Lam t        => Lam P' l' (fixpath' t (S l') (P' ++ [U]) _ ll)
+              | App t1 t2 => App P' l' (fixpath' t1 l' (P' ++ [L]) pr ll ) (fixpath' t2 l' (P' ++ [R]) _ ll)
+              | BVar n eq => match n <? ll with
+                               | true => BVar P' l' 0 _
+                               | false => BVar P' l' (l' - l + n) _
+                             end
+              | FVar n    => FVar P' l' n
             end
-        in fixpath' t l' P' EQ
-    ).
-  omega.
-  omega.
-  omega.
+        in fixpath' t l' P' EQ ll
+    ); omega.
 Defined.
 
-Definition lamFromPath :
-  Path -> nat.
-  refine (fix lamFromPath' (P : Path) : nat :=
-            match P with
-              | [] => 0
-              | x :: xs => let l := (lamFromPath' xs)
-                           in match x with
-                                | U => S l
-                                | _ => l
-                              end
-            end
-         ).
-Defined.
+(* lamInPath : is an auxiliary function that returns a number of
+  lambda nodes in a given path
+*)
+Fixpoint lamInPath (P : Path) : nat :=
+  match P with
+    | [] => 0
+    | x :: xs => let l := (lamInPath xs)
+                 in match x with
+                      | U => S l
+                      | _ => l
+                    end
+  end.
 
-Definition eqq : Role -> Role -> bool.
-  refine (
-      fun r1 r2 => match r1 with
-                     | U => match r2 with
-                              | U => true
-                              | _ => false
-                            end
-                     | L => match r2 with
-                              | L => true
-                              | _ => false
-                            end
-                     | R => match r2 with
-                              | R => true
-                              | _ => false
-                            end
-                   end
-    ).
-Defined.
+(* An equality function for Role *)
+Definition eqq (r1 r2 : Role) : bool :=
+  match r1 with
+    | U => match r2 with
+             | U => true
+             | _ => false
+           end
+    | L => match r2 with
+             | L => true
+             | _ => false
+           end
+    | R => match r2 with
+             | R => true
+             | _ => false
+           end
+  end.
 
-Definition substsubterm1 :
+(* An auxiliary funciton for linearSubstitution function *)
+Definition linearSubstitution1 :
   forall {p p1 : Path} {l l1 : nat}
                            (p1' : Path)
                            (t : TermT p l)
                            (T : TermT p1 l1)
-                           (eq : l >= l1),
+                           (eq : l >= l1)
+                           (ll : nat),
             option (TermT p l).
   refine(
-      fix substsubterm' {p p1: Path} {l l1 : nat}
-                           (p1' : Path)
-                           (t : TermT p l)
-                           (T : TermT p1 l1)
-                           (eq : l >= l1)
-            : option (TermT p l) :=
-            match p1' with
-              | [] => Some (fixpath p l T _)
-              | x :: xs => match x with
-                             | U => match t with
-                                      | Lam _ _ t => match substsubterm' xs t T _ with
-                                                       | None => None
-                                                       | Some t => Some (Lam p l t)
-                                                     end
-                                      | _ => None
-                                    end
-                             | L => match t with
-                                      | App _ _ t1 t2 => match substsubterm' xs t1 T _ with
-                                                       | None => None
-                                                       | Some t1 => Some (App p l t1 t2)
-                                                         end
-                                      | _ => None
-                                    end
-                             | R => match t with
-                                      | App _ _ t1 t2 => match substsubterm' xs t2 T _ with
-                                                       | None => None
-                                                       | Some t2 => Some (App p l t1 t2)
-                                                         end
-                                      | _ => None
-                                    end
-                           end
-            end
-    ).
-  omega.
-  omega.
-  omega.
-  omega.
+      fix linearSubstitution' {p p1: Path} {l l1 : nat}
+          (p1' : Path)
+          (t : TermT p l)
+          (T : TermT p1 l1)
+          (eq : l >= l1)
+          (ll : nat)
+      : option (TermT p l) :=
+        match p1' with
+          | [] => match t with
+                    (* check : we replace BVar *)
+                    (* check : we substitudes the correct variable : i.e. ll == i+1 *)
+                    | BVar i _ => if beq_nat ll (i+1)
+                                  then Some (fixpath p l ll T _)
+                                  else None
+                    (* | BVar i _ => Some (fixpath p l ll T _) *)
+                    | _ => None
+                  end
+          | x :: xs => match x with
+                         | U => match t with
+                                  | Lam t => match linearSubstitution' xs t T _ ll with
+                                               | None => None
+                                               | Some t => Some (Lam p l t)
+                                             end
+                                  | _ => None
+                                end
+                         | L => match t with
+                                  | App t1 t2 => match linearSubstitution' xs t1 T _ ll with
+                                                   | None => None
+                                                   | Some t1 => Some (App p l t1 t2) 
+                                                 end
+                                  | _ => None
+                                end
+                         | R => match t with
+                                  | App t1 t2 => match linearSubstitution' xs t2 T _ ll with
+                                                   | None => None
+                                                   | Some t2 => Some (App p l t1 t2)
+                                                 end
+                                  | _ => None
+                                end
+                       end
+        end
+    ); omega.
 Defined.
 
-Definition substsubterm :
+(* linearSubstitution : is a function that performs a linear substitution.
+  p1 is path to the BVar to be replaced by the subtree indexed by the path p2
+ *)
+Definition linearSubstitution :
   forall {P : Path} {l : nat} (p1 p2 : Path),
   TermT P l -> option (TermT P l).
   refine(
       fun P l p1 p2 t =>
-        let fix substsubterm' {p : Path} {l : nat}
+        let fix linearSubstitution' {p : Path} {l : nat}
                 (p1' p2' : Path)
                 (t : TermT p l)
             : option (TermT p l) :=
@@ -269,255 +280,714 @@ Definition substsubterm :
               | [] => None
               | [R] => match p1' with
                          | L :: ys => match t with
-                                        | App _ _ t1 t2 => match substsubterm1 ys t1 t2 _ with
-                                                             | None => None
-                                                             | Some t1 => Some (App p l t1 t2)
-                                                           end
+                                        | App t1 t2 => match linearSubstitution1 ys t1 t2 _ l with
+                                                         | None => None
+                                                         | Some t1 => Some (App p l t1 t2)
+                                                       end
                                         | _ => None
                                       end
                          | _ => None
                        end
-              | [L] => None
-              | [U] => None
+              | [_] => None
               | x :: xs =>
                 match p1' with
-                             | [] => None
-                             | y :: ys => match eqq x y with
-                                            | true => match x with
-                                                 | U => match t with
-                                                          | Lam _ _ t' => match (substsubterm' ys xs t') with
-                                                                            | None => None
-                                                                            | Some t' => Some (Lam p l t')
-                                                                          end
-                                                          | _ => None
-                                                        end
-                                                 | L =>  match t with
-                                                          | App _ _ t' t'' => match (substsubterm' ys xs t') with
-                                                                                | None => None
-                                                                                | Some t' => Some (App p l t' t'')
-                                                                              end
-                                                          | _ => None
-                                                        end
-                                                 | R =>  match t with
-                                                           | App _ _ t' t'' => match (substsubterm' ys xs t'') with
-                                                                                 | None => None
-                                                                                 | Some t'' => Some (App p l t' t'')
-                                                                               end
-                                                          | _ => None
-                                                         end
-                                                         end
-                                            | false => None
-                                          end
-                           end
+                  | [] => None
+                  | y :: ys => match eqq x y with
+                                 | true => match x with
+                                             | U => match t with
+                                                      | Lam t' => match linearSubstitution' ys xs t' with
+                                                                    | None => None
+                                                                    | Some t' => Some (Lam p l t')
+                                                                  end
+                                                      | _ => None
+                                                    end
+                                             | L =>  match t with
+                                                       | App t' t'' => match linearSubstitution' ys xs t' with
+                                                                         | None => None
+                                                                         | Some t' => Some (App p l t' t'')
+                                                                       end
+                                                       | _ => None
+                                                     end
+                                             | R =>  match t with
+                                                       | App t' t'' => match linearSubstitution' ys xs t'' with
+                                                                         | None => None
+                                                                         | Some t'' => Some (App p l t' t'')
+                                                                       end
+                                                       | _ => None
+                                                     end
+                                           end
+                                 | false => None
+                               end
+                end
             end
-        in substsubterm' p1 p2 t
-    ).
-  auto.   
+        in linearSubstitution' p1 p2 t
+    ); auto.   
 Defined.
 
-Eval compute in substsubterm [U;L;L;U] [U;R] exampleC.
-Eval compute in AppT.
-Eval compute in substsubterm [U;U;L] [U;U;R] AppT.
+Notation "T [| p1 --> p2 |]" := (linearSubstitution p1 p2 T) (at level 0).
 
-Definition TermTEquality :
-  forall {P : Path} {l : nat},
-    TermT P l -> TermT P l -> bool.
+(* An equality function for TermT *)
+Fixpoint TermTEquality {P : Path} {l : nat} (t1 t2 : TermT P l) : bool :=
+  match t1 with
+    | Lam t1 => match t2 with
+                  | Lam t2 =>  TermTEquality t1 t2
+                  | _ => false
+                end
+    | App t1' t1'' => match t2 with
+                        | App t2' t2'' => TermTEquality t1' t2' && TermTEquality t1'' t2''
+                        | _ => false
+                      end
+    | BVar n _ => match t2 with
+                    | BVar m _ => beq_nat m n
+                    | _ => false
+                  end
+    | FVar n => match t2 with
+                  | FVar m => beq_nat m n
+                  | _ => false
+                end
+  end.
+
+(* An equality function for option TermT *)
+Definition OptionTermTEquality {P : Path} {l : nat} (t1 t2 : option (TermT P l)) : bool :=
+  match t1 with
+    | None => match t2 with
+                | None => true
+                | _ => false
+              end
+    | Some t1 => match t2 with
+                   | None => false
+                   | Some t2 => TermTEquality t1 t2
+                 end
+  end.
+
+Example otpe : OptionTermTEquality (AppT [| [U;U;L] --> [U;U;R] |]) (Some AppT') = true. auto. Qed.
+
+Definition exampleC' : Term.
   refine(
-      fix eq {P : Path} {l : nat}
-          (t1 t2 : TermT P l)
-      : bool :=
-        match t1 with
-          | Lam _ _ t1 => match t2 with
-                            | Lam _ _ t2 => eq t1 t2
-                            | _ => false
-                          end
-          | App  _ _ t1' t1'' => match t2 with
-                            | App _ _ t2' t2'' => eq t1' t2' && eq t1'' t2''
-                            | _ => false
-                          end
-          | BVar _ _ n _ => match t2 with
-                            | BVar _ _ m _ => beq_nat m n
-                            | _ => false
-                          end
-          | FVar _ _ n => match t2 with
-                            | FVar _ _ m => beq_nat m n
-                            | _ => false
-                          end
-        end
-    ).
+      Lam [] 0
+          (App [U] 1
+               (Lam [U;L] 1
+                    (App [U;L;U] 2
+                         (Lam [U;L;U;L] 2
+                              (App [U;L;U;L;U] 3
+                                   (BVar [U;L;U;L;U;L] 3 2 _)
+                                   (BVar [U;L;U;L;U;R] 3 0 _)))
+                         (Lam [U;L;U;R] 2 (BVar [U;L;U;R;U] 3 0 _))))
+               (Lam [U;R] 1
+                    (App [U;R;U] 2
+                         (BVar [U;R;U;L] 2 1 _)
+                         (BVar [U;R;U;R] 2 0 _))))
+    ); omega.
 Defined.
 
-Definition OptionTermTEquality :
-  forall {P : Path} {l : nat},
-    option (TermT P l) -> option (TermT P l) -> bool.
-  refine(
-      fix eq  {P : Path} {l : nat}
-          (t1 t2 : option (TermT P l))
-      : bool :=
-        match t1 with
-          | None => match t2 with
-                      | None => true
-                      | _ => false
-                    end
-          | Some t1 => match t2 with
-                      | None => false
-                      | Some t2 => TermTEquality t1 t2
-                    end
-        end
-    ).
-Defined.
+Example exampleCULLUandUR :
+  OptionTermTEquality (exampleC [| [U;L;U;L] --> [U;R] |]) (Some exampleC') = true.
+repeat simpl_eq; auto. Qed.
 
-Eval cbv in  OptionTermTEquality (substsubterm [U;U;L] [U;U;R] AppT) (Some AppT').
-Eval compute in AppT'. Eval compute in AppT.
+Example exampleCULLUandULUR :
+  exampleC [| [U;L;U;L] --> [U;L;U;R] |] = None.
+repeat simpl_eq; auto. Qed.
 
-Theorem substExample :
-  OptionTermTEquality (substsubterm ([U;U;L]) ([U;U;R]) AppT) (Some AppT') = true.
-Proof.
-  unfold substsubterm; unfold substsubterm1; unfold fixpath; unfold eqq;  simpl_eq; auto.
-Qed.
+Example exampleCULLandUR :
+   exampleC [| [U;L;L;U] --> [U;R;R] |] = None.
+simpl_eq; auto. Qed.
 
-(* Theorem substExample' : *)
-(*   substsubterm ([U;U;L]) ([U;U;R]) AppT = Some (AppT'). *)
-(* Proof. *)
-(*   unfold substsubterm; unfold substsubterm1; unfold fixpath; unfold eqq.  simpl_eq. *)
-(*   (* How to unfold AppT'  *) *)
-(*   Admitted. *)
-(* Qed. *)
 
-Theorem exampleCULLUandUR :
-  OptionTermTEquality (substsubterm [U;L;L;U] [U;R] exampleC)
-                      (
-                        Some
-                          (Lam [] 0
-                               (App [U] 1
-                                    (App [U; L] 1
-                                         (Lam [U; L; L] 1
-                                              (Lam [U; L; L; U] 2
-                                                   (App [U; L; L; U; U] 3
-                                                        (BVar [U; L; L; U; U; L] 3 0
-                                                              (Decidable.dec_not_not (1 <= 3) 
-                                                                                     (dec_lt 0 3)
-                                                                                     (fun H : 1 <= 3 -> False =>
-                                                                                        Zge_left 0 3 (proj1 (Nat2Z.inj_ge 0 3) (not_lt 0 3 H))
-                                                                                                 eq_refl)))
-                                                        (BVar [U; L; L; U; U; R] 3 0
-                                                              (Decidable.dec_not_not (1 <= 3) 
-                                                                                     (dec_lt 0 3)
-                                                                                     (fun H : 1 <= 3 -> False =>
-                                                                                        Zge_left 0 3 (proj1 (Nat2Z.inj_ge 0 3) (not_lt 0 3 H))
-                                                                                                 eq_refl))))))
-                                         (Lam [U; L; R] 1
-                                              (BVar [U; L; R; U] 2 1
-                                                    (Decidable.dec_not_not (2 <= 2) 
-                                                                           (dec_lt 1 2)
-                                                                           (fun H : 2 <= 2 -> False =>
-                                                                              Zge_left 1 2 (proj1 (Nat2Z.inj_ge 1 2) (not_lt 1 2 H))
-                                                                                       eq_refl))
-                                              )))
-                                    (Lam [U; R] 1
-                                         (App [U; R; U] 2
-                                              (BVar [U; R; U; L] 2 0
-                                                    (Decidable.dec_not_not (1 <= 2) 
-                                                                           (dec_lt 0 2)
-                                                                           (fun H : 1 <= 2 -> False =>
-                                                                              Zge_left 0 2 (proj1 (Nat2Z.inj_ge 0 2) (not_lt 0 2 H))
-                                                                                       eq_refl)))
-                                              (BVar [U; R; U; R] 2 1
-                                                    (Decidable.dec_not_not (2 <= 2) 
-                                                                           (dec_lt 1 2)
-                                                                           (fun H : 2 <= 2 -> False =>
-                                                                              Zge_left 1 2 (proj1 (Nat2Z.inj_ge 1 2) (not_lt 1 2 H))
-                                                                                       eq_refl))
-                                              ))))))
-  = true.
-Proof.  unfold substsubterm; unfold substsubterm1; unfold fixpath; unfold eqq;  simpl_eq; auto. Qed.
+(**
+===========================================
+  Transition System for Head Linear Reduction
+ ===========================================
+**)
 
-Theorem exampleCULLandUR :
-  substsubterm [U;L;L;U] [U;R;R] exampleC = None.
-Proof.  unfold substsubterm; unfold substsubterm1; unfold fixpath; unfold eqq;  simpl_eq; auto. Qed.
+(* Context Gamma *)
+Inductive Gamma : Type :=
+| EmptyGamma : Gamma
+(* index (variable) -> argument term -> argument context -> rest of the list *)
+| ConsGamma  : nat -> Path -> Gamma -> Gamma -> Gamma.
 
-(* (**  *)
-(* =========================================== *)
-(* Transition System for Head Linear Reduction *)
-(*  =========================================== *)
-(* *) *)
+(* Incompelete Application List Delta *)
+Inductive Delta : Type :=
+| EmptyDelta : Delta
+| ConsDelta  : Path -> Gamma -> Delta -> Delta.
 
-(* (* Context Gamma *) *)
-(* Inductive Gamma : Type := *)
-(* | EmptyGamma : Gamma *)
-(* (* index (variable) -> argument term -> argument context -> rest of the list *) *)
-(* | ConsGamma  : nat -> Path -> Gamma -> Gamma -> Gamma. *)
-
-(* (* Incompelete Application List Delta *) *)
-(* Inductive Delta : Type := *)
-(* | EmptyDelta : Delta *)
-(* | ConsDelta  : Path -> Gamma -> Delta -> Delta. *)
-
-(* (* Term P l --- is an input term with indexed path *) *)
-(* (* Gamma    --- is a current condext *) *)
-(* (* Delta    --- is a current list of incomplete applications *) *)
+(* Term P l --- is an input term with indexed path *)
+(* Gamma    --- is a current condext *)
+(* Delta    --- is a current list of incomplete applications *)
 (* Inductive HLRState := *)
 (* | HLRStateC : Term -> Path -> nat -> Gamma -> Delta -> HLRState *)
 (* | HLRStuck  : HLRState -> HLRState. *)
 
-(* Definition containsGamma : Gamma -> nat -> option (prod Path Gamma). *)
-(*   refine ( *)
-(*       fix containsDelta' (G : Gamma) (N : nat): option (prod Path Gamma) := *)
-(*         match G with *)
-(*           | EmptyGamma => None *)
-(*           | ConsGamma i p g Gs => *)
-(*             if (beq_nat i N) *)
-(*             then Some (pair p g) *)
-(*             else containsDelta' Gs N *)
-(*         end  *)
-(*     ). *)
-(* Defined. *)
 
-(* Definition hlrStep : *)
-(*   HLRState -> HLRState. *)
-(*   refine ( *)
-(*       fun s => *)
-(*         match s with *)
-(*           | HLRStateC T P L1 G D => *)
-(*             let T' := T [P] *)
-(*             in match T' with *)
-(*               | Some T' => *)
-(*                 match T' with *)
-(*                   | Lam  _ l t => *)
-(*                     match D with *)
-(*                       (* [Lam-Non-Elim] *) *)
-(*                       | EmptyDelta         => HLRStateC T (getpath t) (l+1) G D *)
-(*                       (* [Lam-Elim] *) *)
-(*                       | ConsDelta px gx Ds => *)
-(*                         HLRStateC T (getpath t) (l+1) (ConsGamma (getlamnum T') px gx G) Ds *)
-(*                     end *)
-(*                   | App  _ l t1 t2 => HLRStateC T (getpath t1) l     G (ConsDelta (getpath t2) G D) *)
-(*                   (* BVar? *) *)
-(*                   | BVar _ l i     => *)
-(*                     match containsGamma G i with *)
-(*                       | None => HLRStuck s *)
-(*                       | Some (pair p g) => *)
-(*                         match substsubterm T P p with *)
-(*                           | None => HLRStuck s *)
-(*                           (* BVar *) *)
-(*                           (* TODO: fix variable indexes *) *)
-(*                           | Some t => HLRStateC t P l g D *)
-(*                         end *)
-(*                     end *)
-(*                   (* stuck *) *)
-(*                   | FVar _ l       => HLRStuck s *)
-(*                 end *)
-(*               | None   => HLRStuck s *)
-(*             end *)
-(*           | HLRStuck _ => s *)
-(*         end). *)
-(* Defined. *)
+TODO: fix all with respect to the new definition of subterm
 
-(* Definition exampleCInit : HLRState := *)
-(*   HLRStateC exampleC ([]) 0 EmptyGamma EmptyDelta. *)
+Definition ValidPathLam {P : Path} {l : nat} (t : TermT P l) (p : Path) (l1 : nat)  :=
+  exists t' : TermT (P ++ p) l1,
+    Some (existT (fun x => TermT (P ++ p) x) l1 t') = t [|p|] 
+.
 
-(* Eval compute in hlrStep exampleCInit. *)
-(* Eval compute in hlrStep (hlrStep exampleCInit). *)
-(* Eval compute in hlrStep (hlrStep (hlrStep exampleCInit)). *)
-(* Eval compute in hlrStep (hlrStep (hlrStep (hlrStep exampleCInit))). *)
-(* Eval compute in hlrStep (hlrStep (hlrStep (hlrStep (hlrStep exampleCInit)))). *)
+Check ValidPathLam.
+
+
+(* match t[|p|] with *)
+  (*   | None => False *)
+  (*   | Some (existT l' T') => l1 = l' *)
+  (* end. *)
+
+Inductive HLRState :=
+| HLRStateC :
+    forall (t : Term) (p : Path) (l : nat), ValidPathLam t p l
+                                  -> Gamma -> Delta -> HLRState
+| HLRStuck  : HLRState -> HLRState.
+
+Definition containsGamma : Gamma -> nat -> option (prod Path Gamma).
+  refine (
+      fix containsDelta' (G : Gamma) (N : nat): option (prod Path Gamma) :=
+        match G with
+          | EmptyGamma => None
+          | ConsGamma i p g Gs =>
+            if (beq_nat i N)
+            then Some (pair p g)
+            else containsDelta' Gs N
+        end
+    ).
+Defined.
+
+Definition getpath : forall {P : Path} {l : nat}, TermT P l -> Path := fun P _ _  => P.
+Definition getlamnum : forall {P : Path} {l : nat}, TermT P l -> nat := fun _ l _  => l.
+
+Definition isLam {P : Path} {l : nat} (t : TermT P l)  :=
+  exists t' : TermT (P ++ [U]) (S l), t = Lam P l t'.
+
+Lemma ListTypes :
+  forall (P p1 p2 : Path) (l : nat), TermT ((P ++ p1) ++ p2) l = TermT (P ++ p1 ++ p2) l.
+Proof. intros; rewrite app_assoc; reflexivity. Qed.
+
+
+
+Lemma subtermAss :
+  forall {P : Path} {l : nat} (t : TermT P l) (p1 p2 : Path) (l1 l2: nat),
+    (exists (t1 : TermT (P ++ p1) l1) (t2 : TermT ((P ++ p1) ++ p2) l2),
+       Some (existT (fun x : nat => TermT (P ++ p1) x) l1 t1) = (t) [|p1|] /\ Some (existT (fun x : nat => TermT ((P ++ p1) ++ p2) x) l2 t2) = (t1) [|p2|])
+    -> (exists t3 : TermT (P ++ p1 ++ p2) l2,
+       Some (existT (fun x : nat => TermT (P ++ p1 ++ p2) x) l2 t3) = (t) [|p1 ++ p2|]).
+Proof.
+intros. inversion H as [t1 [t2 [H1 H2]]].
+
+induction p2.
+- assert (E : TermT (P ++ p1 ++ []) l2) by (rewrite app_assoc; assumption).
+  exists E. 
+
+
+  rewrite app_nil_r.
+   rewrite <- app_nil_r.
+
+
+clear H2.
+rewrite <- app_assoc in t2.
+exists t2.  
+
+
+
+Qed.
+  
+Theorem ValidPathLamU :
+  forall {P : Path} {l : nat} (t : TermT P l) (p : Path) (l1 : nat),
+  (exists (t' : TermT (P ++ p) l1),
+    Some (existT (fun x => TermT (P ++ p) x) l1 t') = t [| p |] /\ isLam t' )->
+    exists (t'' : TermT (P ++ p ++ [U]) (S l1)),
+      Some (existT (fun x => TermT (P ++ p ++ [U]) x) (S l1) t'') = t [| p ++ [U] |].
+Proof.
+  intros P l t p l1 H; inversion H as [t' [H1 H2]].
+  unfold isLam in H2; inversion H2 as [T H3].
+  assert (E : P ++ p ++ [U] = (P ++ p) ++ [U]) by (rewrite app_assoc; reflexivity).
+
+  clear H3.
+  rewrite <- E in T.
+  exists T.
+  
+
+  
+  rewrite <- ListTypes.
+  ?????
+  rewrite <- E in T.
+  exists T.
+  rewrite <- app_assoc.
+  
+Qed.
+  
+Definition hlrStep :
+  HLRState -> HLRState.
+  refine (
+      fun s =>
+        match s with
+          | HLRStateC T P E L1 G D =>
+            match T [| P |] with
+                 | Some (existT l T') => match T' with
+                                           | Lam  t =>
+                                             match D with
+                                               (* [Lam-Non-Elim] *)
+                                               | EmptyDelta => HLRStateC T (P ++ [U]) (E + 1) _ G D
+                                               (* [Lam-Elim] *)
+                                               | ConsDelta px gx Ds =>
+                                                 HLRStateC T (P ++ [U]) (l+1) _ (ConsGamma (getlamnum T') px gx G) Ds
+                                             end
+                                | App  t1 t2 => HLRStateC T (P ++ [L]) l _ G (ConsDelta (P ++ [R]) G D)
+                                | BVar i _  =>
+                                  (* check that i+1 <= l; otherwise do nothing *)
+                                  (* TODO unnecessary: l > i by the definition*)
+                                  if i <? l
+                                  then match containsGamma G (l - i -1) with
+                                         (* match containsGamma G index (l - i -1) with *)
+                                         | None => HLRStuck s
+                                         | Some (pair p g) =>
+                                           match T [| P -->  p |] with
+                                             | None => HLRStuck s
+                                             (* BVar *)
+                                             | Some T => HLRStateC T P l _ g D
+                                           end
+                                       end
+                                  else HLRStuck s
+                                | FVar _  => HLRStuck s
+                              end
+                 | None => HLRStuck s
+               end
+          | HLRStuck _ => s
+        end).
+  
+  
+
+Defined.
+
+Definition exampleCInit : HLRState := HLRStateC exampleC ([]) 0 EmptyGamma EmptyDelta.
+
+Fixpoint pathEq (xs ys : Path) : bool :=
+  match xs with
+    | [] => match ys with
+              | [] => true
+              | _ => false
+            end
+    | x :: xs => match ys with
+                   | y :: ys => eqq x y && pathEq xs ys
+                   | [] => false
+                 end
+  end.
+
+Fixpoint gammaEq (g1 g2 : Gamma) : bool :=
+  match g1 with
+    | EmptyGamma => match g2 with
+                      | EmptyGamma => true
+                      | _ => false
+                    end
+    | ConsGamma l1 p1 g11 g12 => match g1 with
+                                   | ConsGamma l2 p2  g21 g22 =>
+                                     beq_nat l1 l2 && pathEq p1 p2 && gammaEq g11 g21 && gammaEq g12 g22
+                                   | _ => false
+                                 end
+  end.
+
+Fixpoint deltaEq (d1 d2 : Delta) : bool :=
+  match d1 with
+    | EmptyDelta => match d2 with
+                      | EmptyDelta => true
+                      | _ => false
+                    end
+    | ConsDelta p1 g1 d1 => match d2 with
+                                   | ConsDelta p2 g2 d2 =>
+                                     pathEq p1 p2 && gammaEq g1 g2 && deltaEq d1 d2
+                                   | _ => false
+                                 end
+  end.
+
+Fixpoint  hlrStateEq (s1 s2 : HLRState) : bool :=
+  match s1 with
+    | HLRStuck s1 => match s2 with
+                       | HLRStuck s2 => hlrStateEq s1 s2
+                       | _ => false
+                     end
+    | HLRStateC T1 P1 L1 G1 D1 => match s2 with
+                                    | HLRStateC T2 P2 L2 G2 D2 =>
+                                      TermTEquality T1 T2 && pathEq P1 P2 && beq_nat L1 L2 &&
+                                             gammaEq G1 G2 && deltaEq D1 D2
+                                    | _ => false
+                                  end
+  end.
+
+Example exampleCIntS1 :
+  hlrStateEq (hlrStep exampleCInit) (HLRStateC exampleC [U] 1 EmptyGamma EmptyDelta) = true.
+simpl_eq; auto. Qed.
+
+Example exampleCIntS2 :
+  hlrStateEq (hlrStep (hlrStep exampleCInit))
+             (HLRStateC exampleC [U; L] 1 EmptyGamma
+                        (ConsDelta [U; R] EmptyGamma EmptyDelta)) = true.
+repeat simpl_eq; auto. Qed.
+
+Example exampleCIntS3 :
+  hlrStateEq (hlrStep (hlrStep (hlrStep exampleCInit)))
+             (HLRStateC exampleC [U; L; U] 2
+                        (ConsGamma 1 [U; R] EmptyGamma EmptyGamma)
+                        EmptyDelta)
+  = true.
+repeat simpl_eq; auto. Qed.
+
+Example exampleCIntS4 :
+  hlrStateEq (hlrStep (hlrStep (hlrStep (hlrStep exampleCInit))))
+             (HLRStateC exampleC [U; L; U;L] 2
+                        (ConsGamma 1 [U; R] EmptyGamma EmptyGamma)
+                        (ConsDelta [U;L;U;R] (ConsGamma 1 [U; R] EmptyGamma EmptyGamma) EmptyDelta))
+  = true.
+repeat simpl_eq; auto. Qed.
+
+(* Example exampleCIntS5 : *)
+(*   hlrStateEq (hlrStep (hlrStep (hlrStep (hlrStep (hlrStep exampleCInit))))) *)
+(*              (HLRStateC *)
+(*                 (Lam [] 0 *)
+(*                      (App [U] 1 *)
+(*                           (Lam [U; L] 1 *)
+(*                                (App [U; L;U] 2 *)
+(*                                     (Lam [U; L; U; L] 2 *)
+(*                                          (App [U; L; U; L; U] 3 *)
+(*                                               (BVar [U; L; U; L; U; L] 3 2 *)
+(*                                                     (Decidable.dec_not_not (3 <= 3) (dec_lt 2 3) *)
+(*                                                                            (fun H : 3 <= 3 -> False => Zge_left 2 3 (proj1 (Nat2Z.inj_ge 2 3) (not_lt 2 3 H)) *)
+(*                                                                                                                 eq_refl))) *)
+(*                                               (BVar [U; L; U; L; U; R] 3 0 *)
+(*                                                     (Decidable.dec_not_not (1 <= 3) (dec_lt 0 3) *)
+(*                                                                            (fun H : 1 <= 3 -> False => Zge_left 0 3 (proj1 (Nat2Z.inj_ge 0 3) (not_lt 0 3 H)) *)
+(*                                                                                                                 eq_refl))))) *)
+(*                                     (Lam [U; L; U; R] 2 *)
+(*                                          (BVar [U; L; U; R; U] 3 0 *)
+(*                                                (Decidable.dec_not_not (1 <= 3) (dec_lt 0 3) *)
+(*                                                                       (fun H : 1 <= 3 -> False => Zge_left 0 3 (proj1 (Nat2Z.inj_ge 0 3) (not_lt 0 3 H)) *)
+(*                                                                                                            eq_refl)))))) *)
+(*                           (Lam [U; R] 1 *)
+(*                                (App [U; R; U] 2 *)
+(*                                     (BVar [U; R; U; L] 2 1 *)
+(*                                           (Decidable.dec_not_not (2 <= 2) (dec_lt 1 2) *)
+(*                                                                  (fun H : 2 <= 2 -> False => Zge_left 1 2 (proj1 (Nat2Z.inj_ge 1 2) (not_lt 1 2 H)) eq_refl))) *)
+(*                                     (BVar [U; R; U; R] 2 0 *)
+(*                                           (Decidable.dec_not_not (1 <= 2) (dec_lt 0 2) *)
+(*                                                                  (fun H : 1 <= 2 -> False => Zge_left 0 2 (proj1 (Nat2Z.inj_ge 0 2) (not_lt 0 2 H)) eq_refl))))))) *)
+(*                 [U; L; U; L] *)
+(*                 2 *)
+(*                 EmptyGamma *)
+(*                 (ConsDelta [U;L;U;R] (ConsGamma 1 [U; R] EmptyGamma EmptyGamma) EmptyDelta)) *)
+(*   = true. *)
+(* repeat simpl_eq; auto. Qed. *)
+
+(**
+=====================
+  General substitution
+=====================
+**)
+
+(* function substitution' is an auxiliary function that is used in function substitution  *)
+Definition substitution' : forall {P P' : Path} {l l' : nat} (P1 : Path) (l1 : nat),
+                         nat -> TermT P  l -> TermT P' l' ->
+                         l > 0 -> l1 >= l' -> S l1 = l -> TermT P1 l1.
+  refine (
+      fix st' {P P' : Path} {l l' : nat} (P1 : Path) (l1 ll : nat) (t : TermT P  l ) (T : TermT P' l')
+          (EQ0 : l > 0) (EQ1 : l1 >= l') (EQ2 : S l1 = l) : TermT P1 l1 :=
+        match t with
+          | Lam t => Lam P1 l1 (st' (P1 ++ [U]) (S l1) ll t T _ _ _)
+          | App t1 t2 => App P1 l1(st'  (P1 ++ [L]) l1 ll t1 T _ _ _) (st' (P1 ++ [R]) l1 ll t2 T _ _ _)
+          | FVar n => FVar P1 l1 n
+          | BVar n _ => _
+        end
+    ); try omega.
+  remember (lt_eq_lt_dec (l - ll - 1) n) as b eqn:E; destruct b as [[b1 | b2] | b3].
+  - destruct l1.
+    apply FVar;  apply n.
+    apply (BVar P1 (S l1) (n-1)); omega.
+  - apply (fixpath P1 l1 l' T EQ1).
+  - apply (BVar P1 l1 n).
+    assert (QQ : n <= l1 -1) by omega.
+    assert (QW : forall p : nat, p + 1 - 1 = p) by  (intros; omega).
+    omega.
+Defined.
+
+(* function substitution performs a general substitution.
+   arguments: term and a path to the redex (to the argument of the redex)
+ *)
+Definition substitution : Term -> Path -> option Term.
+  refine(
+      let fix st {P : Path} {l : nat} (t : TermT P l) (p : Path) : option (TermT P l) :=
+          match p with
+            | [R] => match t with
+                       | App (Lam t) T => Some (substitution' P l l t T _ _ _)
+                       | _ => None
+                     end
+            | U :: p => match t with
+                          | Lam t => match st t p with
+                                       | Some t => Some (Lam P l t)
+                                       | None => None
+                                     end
+                          | _ => None
+                        end
+            | L :: p => match t with
+                          | App t t' => match st t p with
+                                          | Some t => Some (App P l t t')
+                                          | None => None
+                                        end
+                          | _ => None
+                        end
+            | R :: p => match t with
+                          | App t' t => match st t p with
+                                          | Some t => Some (App P l t' t)
+                                          | None => None
+                                        end
+                          | _ => None
+                        end
+            | [] => None
+          end
+      in fun t p => st t p
+    ); try omega.
+Defined.
+
+(* args:
+  - term (куда подставляем)
+  - argument (что подставляем)
+  - index (???)
+*)
+Definition general_substitution : forall {P P1 : Path} {l l1 : nat},
+                                    TermT P l -> TermT P1 l1 -> nat -> l >= l1 -> TermT P l.
+  refine(
+      fix st {P P1 : Path} {l l1 : nat} (t : TermT P l) (T : TermT P1 l1) (i : nat) (EQ : l >= l1) : TermT P l :=
+          match t with
+            | Lam t => Lam P l (st t T i _)
+            | App t1 t2 => App P l (st t1 T i _) (st t2 T i _)
+            | BVar n _ => if beq_nat (l - n - 1) i
+                          then fixpath P l l T _
+                          else t
+            | FVar _ => t
+          end
+    ); try omega.
+Defined.
+
+(* Examples *)
+Definition substex : Term. 
+  refine (
+      Lam [] 0 (BVar [U] 1 0 _)
+    ); omega.
+Defined.
+Definition substex1 : TermT [U;R] 1. 
+  refine (
+      Lam [U;R] 1
+          (App [U;R;U] 2
+               (BVar [U;R;U;L] 2 1 _)
+               (BVar [U;R;U;R] 2 0 _))
+    ); omega.
+Defined.
+Definition substex2 : Term.
+  refine (
+      Lam [] 0
+          (Lam [U] 1
+               (App [U;U] 2
+                    (BVar [U;U;L] 2 1 _)
+                    (BVar [U;U;R] 2 0 _)
+               )
+          )
+    ); omega.
+Defined.
+Example gs1 :
+  TermTEquality (general_substitution substex substex1)
+                (substex2)
+                = true.
+
+
+
+
+
+
+
+
+Notation "A {| p |}" := (substitution A p) (at level 0).
+
+(* Examples *)
+Definition substex : Term. 
+  refine (
+      Lam [] 0
+          (App [U] 1
+               (Lam [U;L] 1
+                    (BVar [U;L;U] 2 0 _))
+               (Lam [U;R] 1
+                    (App [U;R;U] 2
+                         (BVar [U;R;U;L] 2 1 _)
+                         (BVar [U;R;U;R] 2 0 _))))
+    ); omega.
+Defined.Definition substex' : Term. 
+  refine (
+      Lam [] 0
+          (Lam [U] 1
+               (App [U;U] 2
+                    (BVar [U;U;L] 2 1 _)
+                    (BVar [U;U;R] 2 0 _)))
+    ); omega.
+Defined.
+Definition substex1 : Term. 
+  refine (
+      Lam [] 0
+          (App [U] 1
+               (Lam [U;L] 1
+                    (App [U;L;U] 2
+                         (BVar [U;L;U;L] 2 0 _)
+                         (BVar [U;L;U;R] 2 0 _)))
+               (Lam [U;R] 1
+                    (App [U;R;U] 2
+                         (BVar [U;R;U;L] 2 1 _)
+                         (BVar [U;R;U;R] 2 0 _))))
+    ); omega.
+Defined.
+Definition substex1' : Term. 
+  refine (
+      Lam [] 0
+          (App [U] 1
+               (Lam [U;L] 1
+                    (App [U;L;U] 2
+                         (BVar [U;L;U;L] 2 1 _)
+                         (BVar [U;L;U;R] 2 0 _)))
+               (Lam [U;R] 1
+                    (App [U;R;U] 2
+                         (BVar [U;R;U;L] 2 1 _)
+                         (BVar [U;R;U;R] 2 0 _)))
+          )
+    ); omega.
+Defined.
+Example ss' : 
+    OptionTermTEquality
+      (substex {| [U;R] |})
+      (Some substex') = true. auto. Qed.
+Example ss1' : 
+    OptionTermTEquality
+      (substex1 {| [U;R] |})
+      (Some substex1') = true. auto. Qed.
+
+(* Auxiliary functions that computes "size" of the HLR stateSize
+    and thus, enforces termination of expansion function 
+*)
+Fixpoint gammaSize (g : Gamma) : nat :=
+  match g with
+    | EmptyGamma => 0
+    | ConsGamma _ _ _ gs => 1 + gammaSize gs
+  end.
+
+Fixpoint deltaSize (d : Delta) : nat :=
+  match d with
+    | EmptyDelta => 1
+    | ConsDelta _ g' ds => gammaSize g' +  deltaSize ds
+  end.
+
+Fixpoint stateSize (s : HLRState) : nat :=
+  match s with
+    | HLRStuck s => stateSize s
+    | HLRStateC _ _ _ g d => gammaSize g +  deltaSize d
+  end.
+
+(* An expansion function *)
+Definition expansion (s : HLRState)  : option Term :=
+  let fix expansion' (ll : nat) (s : HLRState) {struct ll}  : option Term :=
+      match ll, s with 0%nat, _ => None
+                    | S _, HLRStuck s => None (* TODO : expansion s *)
+                    | S ll, HLRStateC t p l g d =>
+                      match g with
+                        | EmptyGamma =>
+                          match d with
+                            | EmptyDelta => Some t
+                            | ConsDelta p' g' ds => None (* expansion' ll (HLRStateC t p l g' ds) *)
+                          end
+                        | ConsGamma l' p' g' gs =>
+                          (*TODO: incorrect! here have to be:
+                           1) real substitution (not linear)
+                           2) with throughing out the xcanseled nodes *)
+                        (* match t [| p --> p' |] with *)
+                          match t {| p' |} with
+                            | Some t => ???
+                            (* expansion' ll (HLRStateC t p l gs d) *)
+                            | None => None
+                          end
+                      end
+      end
+  in expansion' (stateSize s) s.
+
+Example est1 :
+  OptionTermTEquality (expansion (hlrStep exampleCInit))
+                      (Some exampleC) = true.
+simpl_eq; auto. Qed.
+(**)
+Definition exampleC2 : Term. 
+  refine (
+      Lam [] 0
+          (App [U] 1
+               (Lam [U;L] 1
+                    (App [U;L;U] 2
+                         (BVar [U;L;U;L] 2 1 _)
+                         (BVar [U;L;U;R] 2 0 _)
+                    )
+               )
+               (Lam [U;R] 1
+                    (BVar [U;R;U] 2 0 _))
+          )
+    ); omega.
+Defined.
+
+Example est2 :
+  OptionTermTEquality (expansion (hlrStep (hlrStep exampleCInit)))
+                      (Some exampleC2) = true.
+repeat simpl_eq; auto. Qed.
+
+Example exampleCIntS2 :
+  hlrStateEq (hlrStep (hlrStep exampleCInit))
+             (HLRStateC exampleC [U; L] 1 EmptyGamma
+                        (ConsDelta [U; R] EmptyGamma EmptyDelta)) = true.
+repeat simpl_eq; auto. Qed.
+
+Example exampleCIntS3 :
+  hlrStateEq (hlrStep (hlrStep (hlrStep exampleCInit)))
+             (HLRStateC exampleC [U; L; U] 2
+                        (ConsGamma 1 [U; R] EmptyGamma EmptyGamma)
+                        EmptyDelta)
+  = true.
+repeat simpl_eq; auto. Qed.
+
+Definition exampleC : Term. 
+  refine (
+      Lam [] 0
+          (App [U] 1
+               (Lam [U;L] 1
+                    (App [U;L;U] 2
+                         (BVar [U;L;U;L] 2 0 _)
+                         (Lam [U;L;U;R] 2 (BVar [U;L;U;R;U] 3 0 _))
+                    )
+               )
+               (Lam [U;R] 1
+                    (App [U;R;U] 2
+                         (BVar [U;R;U;L] 2 1 _)
+                         (BVar [U;R;U;R] 2 0 _)
+                    )
+               )
+          )
+    ); omega.
+Defined.
+
+
+(**==============
+        Head Redex
+     ==============
+ **)
+Definition headRedex : Term -> option Path.
+  refine(
+      let fix hr {P : Path} {l : nat} (T : TermT P l) : option Path :=
+          match T with
+            | App t _ => match t with
+                             | Lam _ => Some P
+                             | App _ _ => hr t
+                             | _ => None
+                           end
+            | Lam t => hr t
+            | _ => None
+          end
+      in fun t => hr t
+    ). Defined.
+
+Example hreC : headRedex exampleC = Some [U]. auto. Qed.
+
